2pm

temp/Spec.Claim.Capabilities.fst
@@ -1,47 +1,28 @@
 module Spec.Claim.Capabilities
 
-open FStar.Seq
 open Spec.Claim
 open Spec.Claim.Metadata
 open Spec.Claim.Keys
-
-type key = bytes
-
-assume val sharedSecret : k1: key -> k2: key -> Tot key
-
-
-assume val h1: 'a -> bytes
-assume val h2: 'a -> bytes
-assume val h3: 'a -> bytes
-assume val h4: 'a -> bytes
+open Spec.Claim.Common
 
 type kv (a: eqtype) (b:eqtype) = 
   |MkKV : key: a -> value : b -> kv a b      
 
-assume val vrf: bytes -> (tuple2 (bytes) (bytes))
-assume val enc : key: bytes -> plain: bytes -> Tot(bytes)
-assume val dec: key: bytes -> ciphered: bytes -> Tot bytes
-assume val lemmaEncDec : key: bytes -> plain: bytes -> Lemma (ensures( plain =  (let cipherText = enc key plain in 
-                                                                        dec key cipherText )))
-assume val getTime: unit -> time
-
-
-
 
 val claimEncoding : 
   privateKeyVRF: bytes -> 
-  nonce: nat -> 
-  claim_label: string -> 
-  claim_body : string -> Tot (tuple2 (bytes) (kv bytes bytes)) 
+  nonce: bytes -> 
+  claim: claim -> Tot (tuple2 (bytes) (kv bytes bytes)) 
 
 let claimEncoding privateKeyVRF nonce claim = 
-  let claim_label = getClaimLabel claim in 
-  let claim_body = getClaimBosy claim in 
-  let ncl = concat nonce claim_label in 
+  let claimLabel = getClaimLabel claim in
+  let claimLabel = toBytes claimLabel in  
+  let claimBody = getClaimBody claim in 
+  let ncl = concat nonce claimLabel in 
   let k, proof = vrf ncl in 
   let l = h1 k in 
   let ke = h2 k in 
-  let c = enc ke (concat proof claim_body) in 
+  let c = enc ke (concat proof claimBody) in 
   (k, MkKV l c)
 
 val encodeCapability : privateKeyDH : key -> 
