temp/Spec.Claim.ClaimChain.fst
@@ -4,29 +4,11 @@ open FStar.Seq
 open Spec.Claim
 open SkipList2.Statement
 
-open HashFunction
-open FStar.Constructive
-
 open Spec.Claim.Metadata
 open Spec.Claim.Keys
 open Spec.Claim.Capabilities
-
-
-let bytes =  seq FStar.UInt8.t
-
-type time = nat
-
-assume val sign : input: bytes -> Tot bytes
-assume val verify : signature: bytes -> data: bytes -> Tot bool
-
-assume val toBytes: input : 'a ->Tot bytes
-assume val concat: bytes-> bytes -> bytes
-
-assume val signVerif: input: bytes -> 
-  Lemma 
-  (ensures (verify (sign input) input == true ))
-
-assume val random: unit -> Tot bytes
+open Spec.Claim.Common
+open Spec.Claim.MerkleTree
 
 type claimChainBlock  = 
 	|InitClaimChain : 
@@ -37,27 +19,27 @@ type claimChainBlock  =
 			claimsCiphered: bytes -> 
 			state: bytes -> (* id + hash + time *)
 			hashPrevious:bytes -> 
-      signature :bytes -> 
-    ->    
-			claimChainBlock f
+      signature :bytes ->    
+			claimChainBlock
 
 val cipherClaims: cls: list claim -> 
-  privateKeyVRF: bytes -> Tot list bytes
+  privateKeyVRF: bytes -> ML (list (tuple2 (bytes) (kv bytes bytes)))
 
 let cipherClaims cls privateKeyVRF= 
     let nonce = random () in 
     let f = claimEncoding privateKeyVRF nonce in 
-    List.map cls f
+    List.map f cls
 
+    (*)
 val generateBlockGenesis: (* self signed*) meta: metadata ->k: nat ->  cls: list claim{length cls = pow2 k} -> claimChainBlock
 
-let generateBlockGenesis meta cls = 
+let generateBlockGenesis meta  k cls = 
     let id = 0 in 
     let nonce = random () in 
     let t = getTime () in 
     let key = keySearchPkVRF metadata.keys in 
-    let claimsCiphers = cipherClaims cls key in 
-    let hashMerkleTree = merkleListGeneration #claim k cls in 
+    let claimsCiphered = cipherClaims cls key in 
+    let hashMerkleTree = merkleListGeneration #claim k claimsCiphered in 
     let state = concat (concat (toBytes id) (toBytes nonce)) (concat (toBytes time) (hashMerkleTree)) in 
     let hashPrevious = createEmpty 0 in 
       let c1 = concat (toBytes id) (toBytes nonce) in 
@@ -67,7 +49,7 @@ let generateBlockGenesis meta cls =
       let c5 = concat c4 state in 
       let c6 = concat c5 hashPrevious in 
     let signature = enc (keySearchPkSig metadata.keys) c6  in  
-    InitClaimChain id nonce t meta claimsCiphers state hashPrevious signature
+    InitClaimChain id nonce t meta claimsCiphered state hashPrevious signature
 
 val generateBlock: bl: claimChainBlock -> k: nat -> cls : list claim {length cls = pow2 k } -> claimChainBlock
 
@@ -75,14 +57,14 @@ let generateBlock bl k cls =
     let id = (bl.id + 1) in 
     let nonce = random () in 
     let t = getTime () in 
-    let metadata = bl.metadata in 
+    let metadata = bl.meta in 
     let key = keySearchPkVRF metadata.keys in 
-    let claimsCiphers = cipherClaims cls key in 
+    let claimsCiphered = cipherClaims cls key in 
     let hashMerkleTree = merkleListGeneration #claim k cls in 
     let state = concat (concat (toBytes id) (toBytes nonce)) (concat (toBytes time) (hashMerkleTree)) in 
       let c1 = concat (toBytes bl.id) (toBytes bl.nonce) in 
-      let c2 = concat c1 (toBytes bl.time) in 
-      let c3 = concat c2 (toBytes bl.metadata) in 
+      let c2 = concat c1 (toBytes bl.t) in 
+      let c3 = concat c2 (toBytes bl.meta) in 
       let c4 = concat c3 bl.claimsCiphered in 
       let c5 = concat c4 bl.state in 
       let c6 = concat c5 bl.hashPrevious in 
@@ -94,7 +76,7 @@ let generateBlock bl k cls =
       let c5 = concat c4 state in 
       let c6 = concat c5 hashPrevious in 
     let signature = enc (keySearchPkSig metadata.keys) c6  in   
-    InitClaimChain id nonce t meta claimsCiphers state hashPrevious signature
+    InitClaimChain id nonce t metadata claimsCiphered state hashPrevious signature
 
     
 
