temp/Spec.Claim.fst
@@ -1,28 +1,9 @@
 module Spec.Claim
 
 open FStar.Seq
-open SkipList2.Statement
-open SkipList2.Insertion2
-open SkipList2.Properties
-open SkipList2.Search
-
-
-open Spec.Claim.Key
-
-
-assume val sign : input: bytes -> bytes
-assume val verify : signature: bytes -> data: bytes -> Tot bool
-
-assume val toBytes: input : 'a -> bytes
-assume val concat: bytes-> bytes -> bytes
-
-assume val signVerif: input: bytes -> 
-	Lemma 
-	(ensures (verify (sign input) input == true ))
-
-(* Authenticity of information *)
-
-type time = nat
+open Spec.Claim.Keys
+open Spec.Claim.Common
+open Spec.Claim.Metadata
 
 type claim = 
 	|InitClaim: 
@@ -49,20 +30,20 @@ type claim =
 		id: bytes -> 
 		signature : bytes{verify signature id}-> claim
 
-val getClaimLabel: cl: claim -> bytes
+val getClaimLabel: cl: claim -> string
 let getClaimLabel cl = 
 	match cl with
-	| InitClaim  label _ _ -> timeStamp
-	| KeyBindingClaim  label _ _ _ -> timeStamp
-	| ClaimChainState  label _ _ _  -> timeStamp
-	| Revocation label _ _ -> timeStamp
+	| InitClaim  label _ _ _ -> label
+	| KeyBindingClaim  label _ _ _ _ -> label
+	| ClaimChainState  label _ _ _ _  -> label
+	| Revocation label _ _ _-> label
 
 assume val getClaimBody: cl: claim -> bytes
 
 val getClaimTimeStamp: cl: claim -> time
 let getClaimTimeStamp cl = 
 	match cl with
-	| InitClaim _ timeStamp _  -> timeStamp
-	| KeyBindingClaim _ timeStamp _ _ -> timeStamp
-	| ClaimChainState _ timeStamp _ _  -> timeStamp
-	| Revocation _ timeStamp _ -> timeStamp
+	| InitClaim _ timeStamp _ _  -> timeStamp
+	| KeyBindingClaim _ timeStamp _ _ _ -> timeStamp
+	| ClaimChainState _ timeStamp _ _ _ -> timeStamp
+	| Revocation _ timeStamp _ _ -> timeStamp
