temp/Spec.Claim.Claim.fst
@@ -1,0 +1,11 @@
+module Spec.Claim.Claim
+
+open Spec.Claim.Capabilities
+open Spec.Claim.Common
+open Spec.Claim.ClaimChain
+open Spec.Claim
+open Spec.Claim.Keys
+open Spec.Claim.Metadata
+open Spec.Claim.MerkleTree
+
+
