temp/Spec.Claim.Common.fst
@@ -1,0 +1,36 @@
+module Spec.Claim.Common
+
+open FStar.Seq
+
+type bytes = seq nat
+type time = nat
+type key = bytes
+
+assume val toBytes: input : 'a ->Tot bytes
+assume val concat: bytes-> bytes -> bytes
+
+assume val sharedSecret : k1: key -> k2: key -> Tot key
+
+assume val hash: bytes  -> bytes
+assume val h1: bytes -> bytes
+assume val h2: bytes -> bytes
+assume val h3: bytes -> bytes
+assume val h4: bytes -> bytes
+
+assume val vrf: bytes -> (tuple2 (bytes) (bytes))
+assume val enc : key: bytes -> plain: bytes -> Tot(bytes)
+assume val dec: key: bytes -> ciphered: bytes -> Tot bytes
+assume val lemmaEncDec : key: bytes -> plain: bytes -> Lemma (ensures( plain =  (let cipherText = enc key plain in 
+                                                                        dec key cipherText )))
+
+
+assume val getTime: unit -> time
+assume val random: unit -> Tot bytes
+
+
+assume val sign : input: bytes -> Tot bytes
+assume val verify : signature: bytes -> data: bytes -> Tot bool
+assume val signVerif: input: bytes -> 
+  Lemma 
+  (ensures (verify (sign input) input == true ))
+
